

# Math 115E Activity 16

## Chapter 5 Factoring Quadratics Part 2

### How to factor quadratic equations

#### Quadratic factoring when $a = 1$ :

When factoring, the form  $x^2 + bx + c$  can be factored as  $(x + m)(x + n)$   
Start with real numbers  $m$  and  $n$  so:  
they both multiply to  $c$  and both add to  $b$   
There is not a value in front of either  $x$

#### Quadratic factoring when $a \neq 1$ :

When factoring, the form  $ax^2 + bx + c$  can be factored as  $(px + m)(qx + n)$   
Start with two real numbers such that:  
multiply to  $a \cdot c$  and yet add to  $b$   
then we re-group the terms and factor

**Example:** We want to solve  $3x^2 - 11x + 10$  by factoring

**Step 1:** Find the factors of  $3 * 10 = 30$  that add up to  $-11$ , (Write the factors if needed)

**Step 2:** The factors of 30 are:  $\pm(1, 30), \pm(2, 15), \pm(3, 10), \pm(5, 6)$ ,  
so the pair that adds to  $-11$  is  $-5$  and  $-6$

**Step 3:** Rewrite the quadratic:  $3x^2 + (-6x - 5x) + 10 = 0$

**Step 4:** Regroup so that each group has a common factor:  $(3x^2 - 6x) + (-5x + 10) = 0$

**Step 5:** Factor out a common term:  $(3x)(x - 2) - 5(x - 2) = 0$

**Step 6:** Factor again with the  $x - 2$  term:  $(3x - 5)(x - 2) = 0$

**Step 7:** Solve for  $x$ , so we get  $3x - 5 = 0$  and  $x - 2 = 0$ , giving us  $x = \frac{5}{3}$  and  $x = 2$

**DONE:** So starting with  $3x^2 - 11x + 10 = 0$ , we get  $(3x - 5)(x - 2) = 0$

**NOTE:** If we aren't able to factor out a common term or we don't get the same expression in both parentheses in Step 5, then go back to Step 3 and swap the factor pair.

### Factor the following quadratic equations

#1  $x^2 + 9x + 14 = 0$

#7  $9x^2 - 27x + 18 = 0$

#2  $x^2 - 8x + 7 = 0$

#8  $4x^2 - 13x + 10 = 0$

#3  $x^2 + x - 30 = 0$

#9  $2x^2 - 13x - 7 = 0$

#4  $3x^2 + 10x + 8 = 0$

#10  $4x^2 + 20x + 25 = 0$

#5  $2x^2 - 9x + 10 = 0$

#11  $3x^2 - 19x + 20 = 0$

#6  $2x^2 - 6x - 20 = 0$

#12  $8x^2 - 6x - 9 = 0$

## How to use the Quadratic Formula

**The Quadratic Formula:**

*If we are given any polynomial, which may not be factorable, in the form  $ax^2 + bx + c = 0$*

*We can solve this by using the quadratic formula  $x = \frac{-b \pm \sqrt{b^2 - 4ac}}{2a}$*

*We will either get 0, 1 or 2 solutions for the  $x$ -values*

**Example:** We want to solve  $3x^2 - 11x + 10$  by using the Quadratic Formula

**Step 1:** Identify the given coefficients:  $a = 3, b = -11, c = 10$

**Step 2:** Plug these into the formula:  $x = \frac{-(-11) \pm \sqrt{(-11)^2 - 4(3)(10)}}{2(3)}$

**Step 3:** Simplify as much as we can  $x = \frac{-11 \pm \sqrt{121 - 120}}{6} \rightarrow x = \frac{11 \pm 1}{6}$

**Step 4:** Obtain the solutions:  $x = \frac{11 \pm 1}{6}$ , so  $x_1 = \frac{11 + 1}{6} = \frac{12}{6} = 2$  and  $x_2 = \frac{11 - 1}{6} = \frac{10}{6} = \frac{5}{3}$

**DONE:** So starting with  $3x^2 - 11x + 10 = 0$ , we get  $x = \frac{5}{3}$  and  $x = 2$ , which is the same as before!

## Solve the following quadratic equations

#1  $x^2 + 9x + 14 = 0$

#7  $4x^2 - 13x + 10 = 0$

#2  $x^2 + 4x + 2 = 0$

#8  $4x^2 + 20x + 25 = 0$

#3  $x^2 + 2x - 1 = 0$

#9  $10x^2 + 10x - 10 = 0$

#4  $x^2 + x - 30 = 0$

#10  $8x^2 - 6x - 9 = 0$

#5  $2x^2 - 6x + 3 = 0$

#11  $4x^2 - 12x + 3 = 0$

#6  $2x^2 - 9x + 10 = 0$

#12  $2x^2 + 5x - 4 = 0$